@prefix rdf: <http://www.w3.org/1999/02/22-rdf-syntax-ns#> .
@prefix rdfs: <http://www.w3.org/2000/01/rdf-schema#>.
@prefix owl: <http://www.w3.org/2002/07/owl#> .
@prefix xsd: <http://www.w3.org/2001/XMLSchema#> .
@prefix carml: <http://carml.taxonic.com/carml/> .
@prefix rr: <http://www.w3.org/ns/r2rml#> .
@prefix rml: <http://semweb.mmlab.be/ns/rml#> .

carml:
	a owl:Ontology ;
	rdfs:label "CARML RML extension vocabulary"@en ;
	rdfs:comment "This vocabulary defines terms that extend the RML specification."@en ;
	owl:imports
		rr: ,
		rml: ;
.

carml:Stream a owl:Class ;
	rdfs:label "Stream"@en ;
	rdfs:isDefinedBy carml: ;
	rdfs:comment "A stream is a sequence of data."@en ;
.

carml:streamName a owl:DatatypeProperty ;
	rdfs:domain carml:Stream ;
	rdfs:isDefinedBy carml: ;
	rdfs:comment "A name to identify a stream."@en ;
.

carml:FileSource a owl:Class ;
	rdfs:label "FileSource"@en ;
	rdfs:isDefinedBy carml: ;
	rdfs:comment "A file based source."@en ;
.

carml:url a owl:DatatypeProperty ;
	rdfs:label "url"@en ;
	rdfs:domain carml:FileSource ;
	rdfs:range xsd:string ;
	rdfs:isDefinedBy carml: ;
	rdfs:comment "A string referencing the location of the FileSource"@en ;
.

carml:XmlDocument a owl:Class ;
	rdfs:label "XmlDocument"@en ;
	rdfs:subClassOf carml:FileSource ;
	rdfs:isDefinedBy carml: ;
	rdfs:comment "A FileSource that is an XML document"@en ;
.

carml:declaresNamespace a owl:ObjectProperty ;
	rdfs:label "declaresNamespace"@en ;
	rdfs:domain carml:XmlDocument ;
	rdfs:range carml:Namespace ;
	rdfs:isDefinedBy carml: ;
	rdfs:comment "A namespace declaration that is used to support namespaces in XML document references."@en ;
.

carml:Namespace a owl:Class ;
	rdfs:label "Namespace"@en ;
	rdfs:isDefinedBy carml: ;
	rdfs:comment "A document namespace."@en ;
.

carml:namespacePrefix a owl:DatatypeProperty ;
	rdfs:label "namespacePrefix"@en ;
	rdfs:domain carml:Namespace ;
	rdfs:range xsd:string ;
	rdfs:isDefinedBy carml: ;
	rdfs:comment "The prefix value of a namespace."@en ;
.

carml:namespaceName a owl:DatatypeProperty ;
	rdfs:label "namespaceName"@en ;
	rdfs:domain carml:Namespace ;
	rdfs:range xsd:string ;
	rdfs:isDefinedBy carml: ;
	rdfs:comment "The name value of a namespace."@en ;
.

carml:MultiTermMap a owl:Class ;
	owl:deprecated true ;
	rdfs:label "MultiTermMap"@en ;
	rdfs:isDefinedBy carml: ;
	rdfs:comment "A function that generates a collection of RDF terms from a logical source"@en ;
.

carml:MultiObjectMap a owl:Class ;
	owl:deprecated true ;
	rdfs:label "MultiObjectMap"@en ;
	rdfs:subClassOf carml:MultiTermMap ;
	rdfs:isDefinedBy carml: ;
	rdfs:comment "An ObjectMap element to generate multiple object components of the (predicate, object) pair from a logical source"@en ;
.

carml:multiReference a owl:DatatypeProperty ;
	owl:deprecated true ;
	rdfs:label "multiReference"@en ;
	# NOTE: currently only supported on a carml:MultiObjectMap .
	rdfs:domain carml:MultiTermMap ;
	rdfs:range xsd:string ;
	rdfs:isDefinedBy carml: ;
	rdfs:comment "A valid expression that evaluates to a collection of values for a subject, predicate, object, or graph, from a logical source."@en ;
.

carml:multiTemplate a owl:DatatypeProperty ;
	owl:deprecated true ;
	rdfs:label "multiTemplate"@en ;
	# NOTE: currently only supported on a carml:MultiObjectMap .
	rdfs:domain carml:MultiTermMap ;
	rdfs:range xsd:string ;
	rdfs:isDefinedBy carml: ;
	rdfs:comment "A template (format string) to specify how to generate a collection of values for a subject, predicate, object, or graph, using one or more references from a logical source."@en ;
.

carml:multiFunctionValue a owl:ObjectProperty ;
	owl:deprecated true ;
	rdfs:label "multiFunctionValue"@en ;
	# NOTE: currently only supported on a carml:MultiObjectMap .
	rdfs:domain carml:MultiTermMap ;
	rdfs:range rr:TriplesMap ;
	rdfs:isDefinedBy carml: ;
	rdfs:comment "A triples map that represents a function execution which results in a collection of values for a subject, predicate, object, or graph, from a logical source."@en ;
.

carml:multiJoinCondition a owl:ObjectProperty ;
	owl:deprecated true ;
	rdfs:label "multiJoinCondition"@en ;
	# NOTE: currently only supported on a carml:MultiObjectMap .
	rdfs:domain carml:MultiTermMap ;
	rdfs:range carml:MultiJoin ;
	rdfs:isDefinedBy carml: ;
	rdfs:comment "Specifies the multi join condition for joining the multiple child values from the logical source with the parent value of the logical source of the parent triples map."@en ;
.

carml:MultiJoin a owl:Class ;
	owl:deprecated true ;
	rdfs:label "MultiJoin"@en ;
	rdfs:subClassOf rr:Join ;
	rdfs:isDefinedBy carml: ;
	rdfs:comment "A join that supports joining multiple child values with a parent expression."@en ;
.

# Add carml:MultiObjectMap to range of rr:objectMap ;
rr:objectMap
	rdfs:range [
		rdf:type owl:Class ;
		owl:unionOf (
			rr:ObjectMap
			rr:RefObjectMap
			carml:MultiObjectMap
		)
	]
.
